wip for easycrypt proofs

compiler/src/printLeak.ml
@@ -8,8 +8,7 @@ let rec pp_leak_e fmt =
   | LEmpty  -> p "ε"
   | LIdx _i -> p "ι"
   | LAdr _a -> p "α"
-  | LSub s  -> fprintf fmt "sub(%a)" (pp_list ", " pp_leak_e) s
-  | Lop _   -> p "w"  
+  | LSub s  -> fprintf fmt "sub(%a)" (pp_list ", " pp_leak_e) s  
 
 let rec pp_tr_p fmt =
   let p s = fprintf fmt "%s" s in
