compiler/lucky13_full_log.ec
@@ -1,0 +1,484 @@
+require import AllCore IntDiv CoreMap List.
+from Jasmin require import JModel.
+
+require import Array128.
+require import WArray128.
+
+
+
+module M = {
+  var leakages : leakages_t
+  
+  proc duplicate_msb_to_all_jasmin (x:W32.t) : W32.t = {
+    var aux: W32.t;
+    
+    var result:W32.t;
+    
+    leakages <- LeakAddr([]) :: leakages;
+    aux <- x;
+    result <- aux;
+    leakages <- LeakAddr([]) :: leakages;
+    aux <- (result `|>>` (W8.of_int 31));
+    result <- aux;
+    return (result);
+  }
+  
+  proc duplicate_msb_to_all_8_jasmin (x:W32.t) : W8.t = {
+    var aux_0: W8.t;
+    var aux: W32.t;
+    
+    var result:W8.t;
+    var temp:W32.t;
+    
+    leakages <- LeakAddr([]) :: leakages;
+    aux <- x;
+    temp <- aux;
+    leakages <- LeakAddr([]) :: leakages;
+    aux <@ duplicate_msb_to_all_jasmin (temp);
+    temp <- aux;
+    leakages <- LeakAddr([]) :: leakages;
+    aux <- temp;
+    result <- (truncateu8 aux);
+    return (result);
+  }
+  
+  proc constant_time_lt_jasmin (a:W32.t, b:W32.t) : W32.t = {
+    var aux: W32.t;
+    
+    var result:W32.t;
+    
+    leakages <- LeakAddr([]) :: leakages;
+    aux <- a;
+    result <- aux;
+    leakages <- LeakAddr([]) :: leakages;
+    aux <- (result - b);
+    result <- aux;
+    leakages <- LeakAddr([]) :: leakages;
+    aux <@ duplicate_msb_to_all_jasmin (result);
+    result <- aux;
+    return (result);
+  }
+  
+  proc constant_time_ge_jasmin (a:W32.t, b:W32.t) : W32.t = {
+    var aux: W32.t;
+    
+    var result:W32.t;
+    
+    leakages <- LeakAddr([]) :: leakages;
+    aux <- a;
+    result <- aux;
+    leakages <- LeakAddr([]) :: leakages;
+    aux <- (result - b);
+    result <- aux;
+    leakages <- LeakAddr([]) :: leakages;
+    aux <- (invw result);
+    result <- aux;
+    leakages <- LeakAddr([]) :: leakages;
+    aux <@ duplicate_msb_to_all_jasmin (result);
+    result <- aux;
+    return (result);
+  }
+  
+  proc constant_time_eq_8_jasmin (a:W32.t, b:W32.t) : W8.t = {
+    var aux_0: W8.t;
+    var aux: W32.t;
+    
+    var result:W8.t;
+    var temp:W32.t;
+    
+    leakages <- LeakAddr([]) :: leakages;
+    aux <- a;
+    temp <- aux;
+    leakages <- LeakAddr([]) :: leakages;
+    aux <- (temp `^` b);
+    temp <- aux;
+    leakages <- LeakAddr([]) :: leakages;
+    aux <- (temp - (W32.of_int 1));
+    temp <- aux;
+    leakages <- LeakAddr([]) :: leakages;
+    aux_0 <@ duplicate_msb_to_all_8_jasmin (temp);
+    result <- aux_0;
+    return (result);
+  }
+  
+  proc rotate_offset_div (rotate_offset:W32.t, md_size:W32.t,
+                          div_spoiler:W32.t, mac_start:W32.t,
+                          scan_start:W32.t) : W32.t = {
+    var aux: W32.t;
+    
+    
+    
+    leakages <- LeakAddr([]) :: leakages;
+    aux <- md_size;
+    div_spoiler <- aux;
+    leakages <- LeakAddr([]) :: leakages;
+    aux <- (div_spoiler `<<` (W8.of_int 23));
+    div_spoiler <- aux;
+    leakages <- LeakAddr([]) :: leakages;
+    aux <- mac_start;
+    rotate_offset <- aux;
+    leakages <- LeakAddr([]) :: leakages;
+    aux <- (rotate_offset - scan_start);
+    rotate_offset <- aux;
+    leakages <- LeakAddr([]) :: leakages;
+    aux <- (rotate_offset + div_spoiler);
+    rotate_offset <- aux;
+    leakages <- LeakAddr([(zlog2 (to_uint (rotate_offset)))]) :: leakages;
+    aux <- (rotate_offset \umod md_size);
+    rotate_offset <- aux;
+    return (rotate_offset);
+  }
+  
+  proc ssl3_cbc_copy_mac_jasmin (out:W64.t, rec:W64.t, orig_len:W32.t,
+                                 md_size:W32.t) : unit = {
+    var aux_1: W8.t;
+    var aux_0: W32.t;
+    var aux: W64.t;
+    
+    var data:W64.t;
+    var mac_end:W32.t;
+    var mac_start:W32.t;
+    var scan_start:W32.t;
+    var temp_32:W32.t;
+    var i:W32.t;
+    var temp:W64.t;
+    var rotated_mac:W8.t Array128.t;
+    var j:W32.t;
+    var temp2_32:W32.t;
+    var mac_started:W8.t;
+    var mac_ended:W8.t;
+    var b:W8.t;
+    var temp_8:W8.t;
+    var temp2_8:W8.t;
+    var rotate_offset:W32.t;
+    var div_spoiler:W32.t;
+    rotated_mac <- witness;
+    leakages <- LeakAddr([(W64.to_uint (rec + (W64.of_int 16)))]) :: leakages;
+    aux <- (loadW64 Glob.mem (W64.to_uint (rec + (W64.of_int 16))));
+    data <- aux;
+    leakages <- LeakAddr([(W64.to_uint (rec + (W64.of_int 4)))]) :: leakages;
+    aux_0 <- (loadW32 Glob.mem (W64.to_uint (rec + (W64.of_int 4))));
+    mac_end <- aux_0;
+    leakages <- LeakAddr([]) :: leakages;
+    aux_0 <- mac_end;
+    mac_start <- aux_0;
+    leakages <- LeakAddr([]) :: leakages;
+    aux_0 <- (mac_start - md_size);
+    mac_start <- aux_0;
+    leakages <- LeakAddr([]) :: leakages;
+    aux_0 <- (W32.of_int 0);
+    scan_start <- aux_0;
+    leakages <- LeakAddr([]) :: leakages;
+    aux_0 <- md_size;
+    temp_32 <- aux_0;
+    leakages <- LeakAddr([]) :: leakages;
+    aux_0 <- (temp_32 + (W32.of_int 256));
+    temp_32 <- aux_0;
+    leakages <- LeakCond((temp_32 \ult orig_len)) :: LeakAddr([]) :: leakages;
+    if ((temp_32 \ult orig_len)) {
+      leakages <- LeakAddr([]) :: leakages;
+      aux_0 <- orig_len;
+      scan_start <- aux_0;
+      leakages <- LeakAddr([]) :: leakages;
+      aux_0 <- (scan_start - temp_32);
+      scan_start <- aux_0;
+    } else {
+      
+    }
+    leakages <- LeakAddr([]) :: leakages;
+    aux_0 <- (W32.of_int 0);
+    i <- aux_0;
+    
+    leakages <- LeakCond((i \ult md_size)) :: LeakAddr([]) :: leakages;
+    
+    while ((i \ult md_size)) {
+      leakages <- LeakAddr([]) :: leakages;
+      aux <- (zeroextu64 i);
+      temp <- aux;
+      leakages <- LeakAddr([]) :: leakages;
+      aux_1 <- (W8.of_int 0);
+      leakages <- LeakAddr([(W64.to_uint temp)]) :: leakages;
+      rotated_mac.[(W64.to_uint temp)] <- aux_1;
+      leakages <- LeakAddr([]) :: leakages;
+      aux_0 <- (i + (W32.of_int 1));
+      i <- aux_0;
+    leakages <- LeakCond((i \ult md_size)) :: LeakAddr([]) :: leakages;
+    
+    }
+    leakages <- LeakAddr([]) :: leakages;
+    aux_0 <- scan_start;
+    i <- aux_0;
+    leakages <- LeakAddr([]) :: leakages;
+    aux_0 <- (W32.of_int 0);
+    j <- aux_0;
+    
+    leakages <- LeakCond((i \ult orig_len)) :: LeakAddr([]) :: leakages;
+    
+    while ((i \ult orig_len)) {
+      leakages <- LeakAddr([]) :: leakages;
+      aux_0 <- mac_end;
+      temp2_32 <- aux_0;
+      leakages <- LeakAddr([]) :: leakages;
+      aux_0 <- (temp2_32 - md_size);
+      temp2_32 <- aux_0;
+      leakages <- LeakAddr([]) :: leakages;
+      aux_0 <@ constant_time_ge_jasmin (i, temp2_32);
+      temp_32 <- aux_0;
+      leakages <- LeakAddr([]) :: leakages;
+      aux_0 <- temp_32;
+      mac_started <- (truncateu8 aux_0);
+      leakages <- LeakAddr([]) :: leakages;
+      aux_0 <- mac_end;
+      temp2_32 <- aux_0;
+      leakages <- LeakAddr([]) :: leakages;
+      aux_0 <@ constant_time_ge_jasmin (i, temp2_32);
+      temp_32 <- aux_0;
+      leakages <- LeakAddr([]) :: leakages;
+      aux_0 <- temp_32;
+      mac_ended <- (truncateu8 aux_0);
+      leakages <- LeakAddr([]) :: leakages;
+      aux <- (zeroextu64 i);
+      temp <- aux;
+      leakages <- LeakAddr([(W64.to_uint (data + temp))]) :: leakages;
+      aux_1 <- (loadW8 Glob.mem (W64.to_uint (data + temp)));
+      b <- aux_1;
+      leakages <- LeakAddr([]) :: leakages;
+      aux_1 <- mac_started;
+      temp_8 <- aux_1;
+      leakages <- LeakAddr([]) :: leakages;
+      aux_1 <- (invw mac_ended);
+      mac_ended <- aux_1;
+      leakages <- LeakAddr([]) :: leakages;
+      aux_1 <- (temp_8 `&` mac_ended);
+      temp_8 <- aux_1;
+      leakages <- LeakAddr([]) :: leakages;
+      aux_1 <- (temp_8 `&` b);
+      temp_8 <- aux_1;
+      leakages <- LeakAddr([]) :: leakages;
+      aux <- (zeroextu64 j);
+      temp <- aux;
+      leakages <- LeakAddr([(W64.to_uint temp)]) :: leakages;
+      aux_1 <- rotated_mac.[(W64.to_uint temp)];
+      temp2_8 <- aux_1;
+      leakages <- LeakAddr([]) :: leakages;
+      aux_1 <- (temp2_8 `|` temp_8);
+      temp2_8 <- aux_1;
+      leakages <- LeakAddr([]) :: leakages;
+      aux_1 <- temp2_8;
+      leakages <- LeakAddr([(W64.to_uint temp)]) :: leakages;
+      rotated_mac.[(W64.to_uint temp)] <- aux_1;
+      leakages <- LeakAddr([]) :: leakages;
+      aux_0 <- (j + (W32.of_int 1));
+      j <- aux_0;
+      leakages <- LeakAddr([]) :: leakages;
+      aux_0 <@ constant_time_lt_jasmin (j, md_size);
+      temp_32 <- aux_0;
+      leakages <- LeakAddr([]) :: leakages;
+      aux <- (zeroextu64 temp_32);
+      temp <- aux;
+      leakages <- LeakAddr([]) :: leakages;
+      aux_0 <- (j `&` (truncateu32 temp));
+      j <- aux_0;
+      leakages <- LeakAddr([]) :: leakages;
+      aux_0 <- (i + (W32.of_int 1));
+      i <- aux_0;
+    leakages <- LeakCond((i \ult orig_len)) :: LeakAddr([]) :: leakages;
+    
+    }
+    leakages <- LeakAddr([]) :: leakages;
+    aux_0 <@ rotate_offset_div (rotate_offset, md_size, div_spoiler,
+    mac_start, scan_start);
+    rotate_offset <- aux_0;
+    leakages <- LeakAddr([]) :: leakages;
+    aux <- (W64.of_int 0);
+    temp <- aux;
+    
+    leakages <- LeakCond(((truncateu32 temp) \ult md_size)) :: LeakAddr(
+    []) :: leakages;
+    
+    while (((truncateu32 temp) \ult md_size)) {
+      leakages <- LeakAddr([]) :: leakages;
+      aux_1 <- (W8.of_int 0);
+      leakages <- LeakAddr([(W64.to_uint (out + temp))]) :: leakages;
+      Glob.mem <- storeW8 Glob.mem (W64.to_uint (out + temp)) aux_1;
+      leakages <- LeakAddr([]) :: leakages;
+      aux <- (temp + (W64.of_int 1));
+      temp <- aux;
+    leakages <- LeakCond(((truncateu32 temp) \ult md_size)) :: LeakAddr(
+    []) :: leakages;
+    
+    }
+    leakages <- LeakAddr([]) :: leakages;
+    aux_0 <- md_size;
+    temp_32 <- aux_0;
+    leakages <- LeakAddr([]) :: leakages;
+    aux_0 <- (temp_32 - rotate_offset);
+    temp_32 <- aux_0;
+    leakages <- LeakAddr([]) :: leakages;
+    aux_0 <- temp_32;
+    rotate_offset <- aux_0;
+    leakages <- LeakAddr([]) :: leakages;
+    aux_0 <@ constant_time_lt_jasmin (rotate_offset, md_size);
+    temp_32 <- aux_0;
+    leakages <- LeakAddr([]) :: leakages;
+    aux <- (zeroextu64 temp_32);
+    temp <- aux;
+    leakages <- LeakAddr([]) :: leakages;
+    aux_0 <- (rotate_offset `&` (truncateu32 temp));
+    rotate_offset <- aux_0;
+    leakages <- LeakAddr([]) :: leakages;
+    aux_0 <- (W32.of_int 0);
+    i <- aux_0;
+    leakages <- LeakAddr([]) :: leakages;
+    aux_0 <- (W32.of_int 0);
+    j <- aux_0;
+    
+    leakages <- LeakCond((i \ult md_size)) :: LeakAddr([]) :: leakages;
+    
+    while ((i \ult md_size)) {
+      
+      leakages <- LeakCond((j \ult md_size)) :: LeakAddr([]) :: leakages;
+      
+      while ((j \ult md_size)) {
+        leakages <- LeakAddr([]) :: leakages;
+        aux_1 <@ constant_time_eq_8_jasmin (j, rotate_offset);
+        temp_8 <- aux_1;
+        leakages <- LeakAddr([]) :: leakages;
+        aux <- (zeroextu64 i);
+        temp <- aux;
+        leakages <- LeakAddr([(W64.to_uint temp)]) :: leakages;
+        aux_1 <- (temp_8 `&` rotated_mac.[(W64.to_uint temp)]);
+        temp_8 <- aux_1;
+        leakages <- LeakAddr([]) :: leakages;
+        aux <- (zeroextu64 j);
+        temp <- aux;
+        leakages <- LeakAddr([(W64.to_uint (out + temp))]) :: leakages;
+        aux_1 <- (loadW8 Glob.mem (W64.to_uint (out + temp)));
+        temp2_8 <- aux_1;
+        leakages <- LeakAddr([]) :: leakages;
+        aux_1 <- (temp2_8 `|` temp_8);
+        temp2_8 <- aux_1;
+        leakages <- LeakAddr([]) :: leakages;
+        aux_1 <- temp2_8;
+        leakages <- LeakAddr([(W64.to_uint (out + temp))]) :: leakages;
+        Glob.mem <- storeW8 Glob.mem (W64.to_uint (out + temp)) aux_1;
+        leakages <- LeakAddr([]) :: leakages;
+        aux_0 <- (j + (W32.of_int 1));
+        j <- aux_0;
+      leakages <- LeakCond((j \ult md_size)) :: LeakAddr([]) :: leakages;
+      
+      }
+      leakages <- LeakAddr([]) :: leakages;
+      aux_0 <- (rotate_offset + (W32.of_int 1));
+      rotate_offset <- aux_0;
+      leakages <- LeakAddr([]) :: leakages;
+      aux_0 <@ constant_time_lt_jasmin (rotate_offset, md_size);
+      temp_32 <- aux_0;
+      leakages <- LeakAddr([]) :: leakages;
+      aux_0 <- (rotate_offset `&` temp_32);
+      rotate_offset <- aux_0;
+      leakages <- LeakAddr([]) :: leakages;
+      aux_0 <- (i + (W32.of_int 1));
+      i <- aux_0;
+      leakages <- LeakAddr([]) :: leakages;
+      aux_0 <- (W32.of_int 0);
+      j <- aux_0;
+    leakages <- LeakCond((i \ult md_size)) :: LeakAddr([]) :: leakages;
+    
+    }
+    return ();
+  }
+}.
+
+equiv l1 : M.constant_time_lt_jasmin ~ M.constant_time_lt_jasmin :
+={M.leakages}
+==> ={M.leakages}.
+proof.
+proc; inline *; sim.
+qed.
+
+equiv l2 : M.constant_time_ge_jasmin ~ M.constant_time_ge_jasmin :
+={M.leakages}
+==> ={M.leakages}.
+proof.
+proc; inline *; sim.
+qed.
+
+equiv l3 : M.constant_time_eq_8_jasmin ~ M.constant_time_eq_8_jasmin :
+={M.leakages}
+==> ={M.leakages}.
+proof.
+proc; inline *; sim.
+qed.
+
+equiv l4 : M.rotate_offset_div ~ M.rotate_offset_div:
+={M.leakages, md_size, div_spoiler, scan_start} /\
+(0 <= (to_uint (mac_start - scan_start)) < 2^8){1} =
+(0 <= (to_uint (mac_start - scan_start)) < 2^8){2} /\
+(2^ 27 <= to_uint div_spoiler < 2^32){1} =
+(2^ 27 <= to_uint div_spoiler < 2^32){2}
+==> ={M.leakages}.
+proof.
+  proc.
+  wp.
+  skip=> />.
+  move=> &1 &2 h1.
+    
+  
+(* mac_start : position of start of tag *)
+equiv l4 : M.rotate_offset_div ~ M.rotate_offset_div:
+={M.leakages} /\
+zlog2 (to_uint (mac_start{1} + (md_size{1} `>>` W8.one `<<` (of_int 24)%W8) - scan_start{1})) =
+zlog2 (to_uint (mac_start{2} + (md_size{2} `>>` W8.one `<<` (of_int 24)%W8) - scan_start{2}))
+(*/\
+zlog2 (to_uint rotate_offset{1}) = zlog2 (to_uint rotate_offset{2})*)
+==> ={M.leakages}.
+proof.
+proc.
+wp.
+skip=> /> &1 &2.
+qed.
+
+(* md_size : mac tag size --> public *)
+(* orig_len : length of record : header + data + mac tag + padding --> public *)
+(* out : mac tag is stored in out --> public *)
+(* rec : whole message including header, message, tag, padding --> public *)
+equiv l_final : M.ssl3_cbc_copy_mac_jasmin ~ M.ssl3_cbc_copy_mac_jasmin :
+={M.leakages, md_size, orig_len, out, rec} /\
+(loadW64 Glob.mem (to_uint (rec + (of_int 16)%W64))){1} =
+(loadW64 Glob.mem (to_uint (rec + (of_int 16)%W64))){2}
+==> ={M.leakages}.
+proof.
+proc.
+wp.
+while (={M.leakages, out, i, j, md_size}).
+inline *; sim.
+conseq (: _ ==> ={M.leakages, i,j, md_size, out}) => //.
+sim 39 39.
+call l4; wp.
+simplify.
+inline *=> />.
++ move=> &1 &2 [h1] [h2] [h3] [h4] h5 l ml sl l' ml' sl' [] [hl] hlog hlog'.
+  split=> //=.
+  + split=> //.
+    rewrite h2. by apply hlog.
+  move=> />. rewrite h2. by apply hlog'.
+simplify.
+wp.
+while (={M.leakages, out, i, j, md_size, orig_len}).
+inline *; sim.
++ move=> &1 &2 [] [h1] [h2] [h3] [h4] [h5] h6 [h7] h8. split=> //=.
+  rewrite h3 h4 h6 h5 h1. split=> //=. admit.
+simplify.
+wp.
+while (={M.leakages, i, md_size}).
++ by sim.
+wp. skip=> />.
+simplify; wp; simplify.
+
+case (md_size{2} + (of_int 256)%W32 \ult orig_len{2}).
++ inline*=> />.
+  move=> &1 &2.
+ admitted.
+
+
