compiler/mod_patch.ec
@@ -1,0 +1,120 @@
+require import AllCore IntDiv CoreMap List.
+from Jasmin require import JModel.
+
+
+
+
+module M = {
+  var leakages : leakages_t
+  
+  proc lzcnt (x:W64.t) : bool * W64.t = {
+    var aux_3: bool;
+    var aux_2: bool;
+    var aux_1: bool;
+    var aux_0: bool;
+    var aux: bool;
+    var aux_4: W64.t;
+    
+    var zf:bool;
+    var result:W64.t;
+    var  _0:bool;
+    var  _1:bool;
+    var  _2:bool;
+    var  _3:bool;
+    
+    leakages <- LeakAddr([]) :: leakages;
+    (aux_3, aux_2, aux_1, aux_0, aux, aux_4) <- LZCNT_64 x;
+     _0 <- aux_3;
+     _1 <- aux_2;
+     _2 <- aux_1;
+     _3 <- aux_0;
+    zf <- aux;
+    result <- aux_4;
+    return (zf, result);
+  }
+  
+  proc verify_mod_const (a:W64.t, b:W64.t) : W64.t = {
+    var aux_0: bool;
+    var aux: W64.t;
+    
+    var result:W64.t;
+    var flag:W64.t;
+    var one:W64.t;
+    var zero:W64.t;
+    var lzbz:bool;
+    var lzb:W64.t;
+    var lzaz:bool;
+    var b_lzb:W64.t;
+    var temp2:W64.t;
+    var temp:W64.t;
+    var b_lzb_1:W64.t;
+    var temp3:W64.t;
+    var res_temp:W64.t;
+    var  _0:W64.t;
+    
+    leakages <- LeakAddr([]) :: leakages;
+    aux <- (W64.of_int 4660);
+    flag <- aux;
+    leakages <- LeakAddr([]) :: leakages;
+    aux <- (W64.of_int 1);
+    one <- aux;
+    leakages <- LeakAddr([]) :: leakages;
+    aux <- (W64.of_int 0);
+    zero <- aux;
+    leakages <- LeakAddr([]) :: leakages;
+    (aux_0, aux) <@ lzcnt (b);
+    lzbz <- aux_0;
+    lzb <- aux;
+    leakages <- LeakAddr([]) :: leakages;
+    aux <- (lzbz ? zero : flag);
+    flag <- aux;
+    leakages <- LeakAddr([]) :: leakages;
+    (aux_0, aux) <@ lzcnt (a);
+    lzaz <- aux_0;
+     _0 <- aux;
+    leakages <- LeakAddr([]) :: leakages;
+    aux <- (lzaz ? one : flag);
+    flag <- aux;
+    leakages <- LeakAddr([]) :: leakages;
+    aux <- b;
+    b_lzb <- aux;
+    leakages <- LeakAddr([]) :: leakages;
+    aux <- (b_lzb `<<` (truncateu8 lzb));
+    b_lzb <- aux;
+    leakages <- LeakAddr([]) :: leakages;
+    aux <- LEA_64 (b_lzb + a);
+    temp2 <- aux;
+    leakages <- LeakAddr([]) :: leakages;
+    aux <- temp2;
+    temp <- aux;
+    leakages <- LeakAddr([]) :: leakages;
+    aux <- (lzb - (W64.of_int 1));
+    lzb <- aux;
+    leakages <- LeakAddr([]) :: leakages;
+    aux <- b;
+    b_lzb_1 <- aux;
+    leakages <- LeakAddr([]) :: leakages;
+    aux <- (b_lzb_1 `<<` (truncateu8 lzb));
+    b_lzb_1 <- aux;
+    leakages <- LeakAddr([]) :: leakages;
+    aux <- LEA_64 (b_lzb_1 + a);
+    temp3 <- aux;
+    leakages <- LeakAddr([]) :: leakages;
+    aux <- ((temp2 \ult b_lzb) ? temp3 : temp);
+    temp <- aux;
+    leakages <- LeakAddr([]) :: leakages;
+    aux <- ((flag = (W64.of_int 1)) ? a : temp);
+    temp <- aux;
+    leakages <- LeakAddr([(W64.ALU.leak_div (temp))]) :: leakages;
+    aux <- (temp \umod b);
+    res_temp <- aux;
+    leakages <- LeakAddr([]) :: leakages;
+    aux <- res_temp;
+    result <- aux;
+    leakages <- LeakAddr([]) :: leakages;
+    aux <- ((flag = (W64.of_int 0)) ? a : result);
+    result <- aux;
+    return (result);
+  }
+}.
+
