compiler/mod_patch_bash_proof.ec
@@ -1,0 +1,24 @@
+require import AllCore IntDiv CoreMap List.
+from Jasmin require import JModel.
+
+require import Mod_patch_bash.
+
+
+lemma lzcnt_zero : forall (w: t), leak_div (w `<<<` leak_div w) = 0.
+admitted.
+
+equiv l2 : M.verify_mod_const ~ M.verify_mod_const : ={M.leakages, b} ==> ={M.leakages}.
+proof.
+  proc.
+  wp=> //=.
+  rewrite /leak_div //=.
+  inline *=> />; wp.
+  simplify. skip=> />.
+  move=> &1 &2 //=.
+  case: ((LZCNT_64 a{1}).`6 = W64.zero) =>//=.
+  (* leading zero of a is 0 *)
+  + move=> h1 />. case: ((LZCNT_64 a{2}).`6 = W64.zero)=> //=.
+    (* leading zero of a is 0 *)
+    + move=> h2 /=. rewrite /LZCNT_64 /leak_div /= in h1. rewrite /LZCNT_64 /leak_div /= in h2.
+      search _ of_int.
+      
