compiler/mod_patch_proof.ec
@@ -1,0 +1,17 @@
+require import AllCore IntDiv CoreMap List.
+from Jasmin require import JModel.
+
+require import Mod_patch.
+
+
+lemma lzcnt_zero : forall w, LZCNT_64 (w << LZCNT_64 w) = 0.
+
+equiv l2 : M.verify_mod_const ~ M.verify_mod_const : ={M.leakages, b} ==> ={M.leakages}.
+proof.
+  proc.
+  wp=> //=.
+  rewrite /leak_div //=.
+  inline *=> />; wp.
+  simplify. skip=> />.
+  move=> &1 &2 //=.
+  
